rustfrontend/BorrowCheckInv.v
@@ -28,10 +28,7 @@ Context {ame: adt_mem_env}.
 
 Notation footprint := (@footprint ame).
 Notation fp_map := (@fp_map ame).
-Notation fp_graph := (@fp_graph ame).
-Notation fp_frame := (@fp_frame ame).
-Notation fp_graph_frame := (@fp_graph_frame ame).
-Notation get_owner_path_frame := (@get_owner_path_frame ame).
+Notation get_owner_path_map := (@get_owner_path_map ame).
 
 (* Section COMP_ENV. *)
 
@@ -75,35 +72,35 @@ Notation get_owner_path_frame := (@get_owner_path_frame ame).
 
 (* End COMP_ENV. *)
 
-Fixpoint mutable_path_footprint (fpgf: fp_graph_frame) (phl: list projection) (fp: footprint) : res bool :=
+Fixpoint mutable_path_footprint (fpg: fp_map) (phl: list projection) (fp: footprint) : res bool :=
   match phl with
   | nil => OK true
   | pj :: l =>
       match pj, fp with
       | proj_deref , fp_box _ fp1 =>          
-          mutable_path_footprint fpgf l fp1
+          mutable_path_footprint fpg l fp1
       | proj_field fid, fp_struct _ fpl =>
           match find_field fid fpl with
           | Some (_, ffp) =>
-              mutable_path_footprint fpgf l ffp
+              mutable_path_footprint fpg l ffp
           | None => Error nil
           end
       | proj_field fid, fp_object _ _ fpl =>
           match find_field fid fpl with
           | Some (_, ffp) =>
-              mutable_path_footprint fpgf l ffp
+              mutable_path_footprint fpg l ffp
           | None => Error nil
           end
       | proj_downcast fid1, fp_enum _ _ fid2 _ fp1 =>
           if ident_eq fid1 fid2 then
-            mutable_path_footprint fpgf l fp1
+            mutable_path_footprint fpg l fp1
           else
             Error nil
       | proj_deref, fp_ref mut _ _ (Some ph2) rebor =>
           match mut with
           | Mutable =>
-              do fp2 <- get_owner_footprint_frame ph2 fpgf;
-              mutable_path_footprint fpgf l fp2
+              do fp2 <- get_owner_footprint_map ph2 fpg;
+              mutable_path_footprint fpg l fp2
           | Immutable =>
               OK false
           end
@@ -112,15 +109,11 @@ Fixpoint mutable_path_footprint (fpgf: fp_graph_frame) (phl: list projection) (f
   end.
 
 
-Definition mutable_spath (sph: spath) (fpgf: fp_graph_frame) : res bool :=
-  let '(fid, (id, phl)) := sph in
-  match nth_error fpgf fid with
-  | Some fpg =>
-      match fpg!id with
-      | Some fp =>
-          mutable_path_footprint fpgf phl fp
-      | _ => Error nil
-      end
+Definition mutable_path (ph: path) (fpg: fp_map) : res bool :=
+  let (id, phl) := ph in
+  match fpg!id with
+  | Some (_,fp) =>
+      mutable_path_footprint fpg phl fp
   | _ => Error nil
   end.
 
@@ -154,20 +147,20 @@ Definition dominators_of_owner_projections (l: list projection) : list (list pro
   filter (fun '(_, s) => in_dec projection_eq proj_deref s) (all_splits l).
 
 
-Inductive reachable_from_dominators (fpgf: fp_graph_frame) : spath -> spath -> Prop :=
-| reachable_from_dominators_intro: forall fid1 fid2 id1 pjl1 id2 pjl dom_pjl suf_pjl vs,
+Inductive reachable_from_dominators (fpg: fp_map) : path -> path -> Prop :=
+| reachable_from_dominators_intro: forall id1 pjl1 id2 pjl dom_pjl suf_pjl vs,
     In (dom_pjl, suf_pjl) (dominators_of_owner_projections pjl) ->
-    get_owner_path_frame (fid1, (id1, pjl1)) fpgf = OK ((fid2, (id2, dom_pjl)), vs) ->
-    reachable_from_dominators fpgf (fid1, (id1, pjl1 ++ suf_pjl)) (fid2, (id2, pjl)).
+    get_owner_path_map (id1, pjl1) fpg = OK ((id2, dom_pjl), vs) ->
+    reachable_from_dominators fpg (id1, pjl1 ++ suf_pjl) (id2, pjl).
     
-Definition fp_ref_views_adequate (fpgf: fp_graph_frame) (tgt: spath) (vs: views) : Prop := 
-  forall ph1, reachable_from_dominators fpgf ph1 tgt ->
-         mutable_spath ph1 fpgf = OK true ->
+Definition fp_ref_views_adequate (fpg: fp_map) (tgt: path) (vs: views) : Prop := 
+  forall ph1, reachable_from_dominators fpg ph1 tgt ->
+         mutable_path ph1 fpg = OK true ->
          In ph1 vs.
 
 (* Note that the precision is conditional. It only holds for the valid
 path. *)
-Definition fp_ref_views_precise (fpgf: fp_graph_frame) (tgt: spath) (vs: views) : Prop := 
+Definition fp_ref_views_precise (fpg: fp_map) (tgt: path) (vs: views) : Prop := 
   forall ph1 tgt1 vs1,
     In ph1 vs ->
     (* If it reaches a target? Consider invalidate some mutable
@@ -180,39 +173,40 @@ Definition fp_ref_views_precise (fpgf: fp_graph_frame) (tgt: spath) (vs: views) 
     (* Actually, it is not definable because we need to do something
     like when invalidating a reference, we need to kill the loans
     related to this reference for other reference.  *)
-    get_owner_path_frame ph1 fpgf = OK (tgt1, vs1) ->
-    tgt = tgt1 /\ mutable_spath ph1 fpgf = OK true.
+    get_owner_path_map ph1 fpg = OK (tgt1, vs1) ->
+    tgt = tgt1 /\ mutable_path ph1 fpg = OK true.
 
 (* We cannot define stack discipline in the context of fp_map because
 we need to show that all the temporary footprint does not point to the
 same location? We need to define this property in the whole fp_graph
 with temporary values. *)
 
-Inductive views_order (fpgf: fp_graph_frame) (sph1 sph2: spath) (vs1 vs2: views) : Prop :=
+
+Inductive views_order (fpg: fp_map) (ph1 ph2: path) (vs1 vs2: views) : Prop :=
 | views_order_immut_mut
-    (IMMUTL: mutable_spath sph1 fpgf = OK false)
-    (MUT: mutable_spath sph2 fpgf = OK true)
+    (IMMUTL: mutable_path ph1 fpg = OK false)
+    (MUT: mutable_path ph2 fpg = OK true)
     (INCL: incl vs2 vs1)
     (NEQ: ~ list_equiv vs1 vs2):
-  views_order fpgf sph1 sph2 vs1 vs2
+  views_order fpg ph1 ph2 vs1 vs2
 | views_order_mut_immut
-    (IMMUTL: mutable_spath sph2 fpgf = OK false)
-    (MUT: mutable_spath sph1 fpgf = OK true)
+    (IMMUTL: mutable_path ph2 fpg = OK false)
+    (MUT: mutable_path ph1 fpg = OK true)
     (INCL: incl vs1 vs2)
     (NEQ: ~ list_equiv vs1 vs2):
-  views_order fpgf sph1 sph2 vs1 vs2
+  views_order fpg ph1 ph2 vs1 vs2
 | views_order_mut_mut
-    (IMMUTL: mutable_spath sph1 fpgf = OK true)
-    (MUT: mutable_spath sph2 fpgf = OK true)
+    (IMMUTL: mutable_path ph1 fpg = OK true)
+    (MUT: mutable_path ph2 fpg = OK true)
     (INCL: incl vs1 vs2 \/ incl vs2 vs1)
     (NEQ: ~ list_equiv vs1 vs2):
-  views_order fpgf sph1 sph2 vs1 vs2
+  views_order fpg ph1 ph2 vs1 vs2
 | views_order_immut_immut
-    (IMMUTL: mutable_spath sph1 fpgf = OK false)
-    (MUT: mutable_spath sph2 fpgf = OK false):
+    (IMMUTL: mutable_path ph1 fpg = OK false)
+    (MUT: mutable_path ph2 fpg = OK false):
   (* The relation between two immutable paths are not important?
   Because they cannot invalidate each other. *)
-  views_order fpgf sph1 sph2 vs1 vs2.
+  views_order fpg ph1 ph2 vs1 vs2.
 
   
 (* The paths that reach the same location should form a total order
@@ -220,13 +214,13 @@ chain. Should we enforce that the views of mutable path must be
 smaller than those of immutable path? Because we have an invariant say
 that all paths in the view is mutable path, then there must be no
 mutable path whose views are greater than some immutable path? *)
-Definition fp_graph_views_inv (fpgf: fp_graph_frame) : Prop :=
+Definition fp_graph_views_inv (fpg: fp_map) : Prop :=
   forall ph1 ph2 tgt vs1 vs2,
     ph1 <> ph2 ->
     (* How to distinguish mutable and immutable path? *)
-    get_owner_path_frame ph1 fpgf = OK (tgt, vs1) ->
-    get_owner_path_frame ph2 fpgf = OK (tgt, vs2) ->
-    views_order fpgf ph1 ph2 vs1 vs2.
+    get_owner_path_map ph1 fpg = OK (tgt, vs1) ->
+    get_owner_path_map ph2 fpg = OK (tgt, vs2) ->
+    views_order fpg ph1 ph2 vs1 vs2.
 
     (* (** In fact, there is no need to compare the views between two *)
     (* immutable path because they cannot affect each other.  *) *)
@@ -290,9 +284,9 @@ point-to owner path. The second is that the views stored in each
 reference must contain all the paths which reach to the point-to
 target via a dominator path. *)
 
-Section FPF_ENV.
+Section FPM_ENV.
 
-Variable fpf: fp_frame.
+Variable fpm: fp_map.
 
 (* We define a new field_offset which returns the starting offset of a
 field that does not consider the alignment. *)
@@ -318,7 +312,7 @@ Inductive fp_ref_loc_wf : footprint -> Prop :=
     fp_ref_loc_wf (fp_enum id tag fid fofs ffp)
 | fp_ref_some_wf: forall ph b ofs fp vs mut 
     (* Reference consistency property *)
-    (GLOC: get_owner_loc_footprint_frame ph fpf = OK (b, ofs, fp))
+    (GLOC: get_owner_loc_footprint_map ph fpm = OK (b, ofs, fp))
     (*TODO: there should be also an invariant about fp which says that fp is fully init, but it is unclear whether we should put it here. *)
     (* It is OK to just say that the views are adequate in fpm instead
     of fp_graph which contains the temporary value, because there
@@ -328,8 +322,8 @@ Inductive fp_ref_loc_wf : footprint -> Prop :=
     (* This adequate property may be redundant for temporary value
     since the fp_ref_views_inv is stronger than this adequacy. But
     this proeprty is required for the reference inside the fp_map.  *)
-    (ADEQUATE: fp_ref_views_adequate fpf ph vs)
-    (PRECISE: fp_ref_views_precise fpf ph vs)
+    (ADEQUATE: fp_ref_views_adequate fpm ph vs)
+    (PRECISE: fp_ref_views_precise fpm ph vs)
     (** TODO: we need to show that all path in vs are valid in fpm *),
     fp_ref_loc_wf (fp_ref mut b ofs (Some ph) vs)
 | fp_ref_none_wf: forall b ofs vs mut,
@@ -341,13 +335,12 @@ Inductive fp_ref_loc_wf : footprint -> Prop :=
 Definition fp_ref_loc_wf_list fpl :=
   Forall fp_ref_loc_wf fpl.
 
-End FPF_ENV.
+End FPM_ENV.
 
-Definition fp_ref_loc_wf_fpf (fpf: fp_frame) : Prop :=
-  forall fid id b ofs ty fp fpm,
-    nth_error fpf fid = Some fpm ->
+Definition fp_ref_loc_wf_fpm (fpm: fp_map) : Prop :=
+  forall id b ofs ty fp,
     fpm ! id = Some (b, ofs, ty, fp) ->
-    fp_ref_loc_wf fpf fp.
+    fp_ref_loc_wf fpm fp.
 
 
 (* Definition fpg_ref_type_inv ce (fpg: fp_graph) : Prop := *)
@@ -368,15 +361,15 @@ the expression and fpm to compute the address.  *)
 
 
 (* The invariant established and preserved by the borrow checking *)
-Record borrow_check_inv (fpf: fp_frame) : Prop :=
-  { borrowck_views_inv: fp_graph_views_inv (fpf_to_fpgf fpf);
+Record borrow_check_inv (fpm: fp_map) : Prop :=
+  { borrowck_views_inv: fp_graph_views_inv fpm;
     (** One alternative is to encode the location invariant of fp_ref
     into views invariant: for all reachable path, if we can compute
     its reached memory location, then this location must be equal to
     the owner location? One (big) problem is that get_owner_path is
     defined on fp_graph instead of fp_map, we cannot compute the
     target location of arbitary path? *)
-    borrowck_fp_ref_loc_inv: fp_ref_loc_wf_fpf fpf; }.
+    borrowck_fp_ref_loc_inv: fp_ref_loc_wf_fpm fpm; }.
 
 
 (* Useful in the proof to store the evaluated value in a fresh temp *)
@@ -394,16 +387,15 @@ fpm, invariant of temp fp w.r.t. fpm and invariant of "for any two
 temp fp, there reachable views must be disjoint" *)
 (* We need to establish invariant for some intermediate state which
 contains some computed values (e.g., creating a reference) *)
-Record borrow_check_inv_snapshot (fpf: fp_frame) (fpgf: fp_graph_frame) (fpl: list footprint) : Prop :=
-  { borrowck_views_inv_snapshot: fp_graph_views_inv fpgf;
-    borrowck_fp_ref_loc_inv_snapshot: fp_ref_loc_wf_fpf fpf;
-    borrowck_fpl_wf: fp_ref_loc_wf_list fpf fpl}.
+Record borrow_check_inv_snapshot (fpm: fp_map) (fpl: list footprint) : Prop :=
+  { borrowck_views_inv_snapshot: fp_graph_views_inv fpm;
+    borrowck_fp_ref_loc_inv_snapshot: fp_ref_loc_wf_fpm fpm;
+    borrowck_fpl_wf: fp_ref_loc_wf_list fpm fpl}.
 
-(** TODO  *)
-Definition borrow_check_fpm_vals_inv (fpf: fp_frame) (vl: list footprint) : Prop :=
-  (* let idl := fresh_PTree_idents fpm (length vl) in *)
-  (* let fpg1 := PTree_Properties.of_list ((PTree.elements (fpm_to_fpg fpm)) ++ (combine idl vl)) in *)
-  borrow_check_inv_snapshot fpf fpf vl.
+(* Definition borrow_check_fpm_vals_inv (fpm: fp_map) (vl: list footprint) : Prop := *)
+(*   let idl := fresh_PTree_idents fpm (length vl) in *)
+(*   let fpg1 := PTree_Properties.of_list ((PTree.elements fpm) ++ (combine idl vl)) in *)
+(*   borrow_check_inv_snapshot fpm fpg1 vl. *)
 
 (* Lemma borrow_check_fpg_vals_inv_empty: forall fpm, *)
 (*     borrow_check_fpm_vals_inv fpm nil -> *)
@@ -418,7 +410,7 @@ Definition fpm_to_tenv (fpm: fp_map) : typenv :=
 Section COMP_ENV.
 
 Variable ce: composite_env.
-Variable te: list typenv.
+Variable te: typenv.
 (** Move it to Rusttypes.v  *)
 
 (* We define a new field_offset which returns the starting offset of a
@@ -487,7 +479,7 @@ callee. In a well-formed footprint/fp_map, it should not appear. *)
 (*     (LOCEQ: get_owner_loc_footprint_map ph fpm = OK (b, ofs, fp)),     *)
 (*     wt_footprint (Treference org mut ty) (fp_ref mut b ofs (Some ph) vs) *)
 | wt_fp_ref_some: forall ty b ofs org mut vs ph pty
-    (WTPH: wt_spath ce te ph = OK pty)
+    (WTPH: wt_path ce te ph = OK pty)
     (TYEQ: type_eq_except_origins ty pty = true),
     wt_footprint (Treference org mut ty) (fp_ref mut b ofs (Some ph) vs)
 | wt_fp_ref_none: forall ty b ofs org mut vs,
@@ -506,78 +498,74 @@ Definition wt_footprint_list tyl fpl :=
 
 End COMP_ENV.
 
-Definition fpf_to_tenv (fpf: fp_frame) := map fpm_to_tenv fpf.
-
-Definition wt_fpf ce (fpf: fp_frame) : Prop :=
-  forall fid fpm id b ofs ty fp,
-    nth_error fpf fid = Some fpm ->    
+Definition wt_fpm ce (fpm: fp_map) : Prop :=
+  forall id b ofs ty fp,
     fpm ! id = Some (b, ofs, ty, fp) ->
-    wt_footprint ce (fpf_to_tenv fpf) ty fp.
+    wt_footprint ce (fpm_to_tenv fpm) ty fp.
 
 
 (** Properties of get/set footprint map  *)
-Lemma get_owner_loc_footprint_frame_wt ce: forall sph fpf b ofs fp,
-    get_owner_loc_footprint_frame sph fpf = OK (b, ofs, fp) ->
-    wt_fpf ce fpf ->
-    exists ty, wt_spath ce (fpf_to_tenv fpf) sph = OK ty
-          /\ wt_footprint ce (fpf_to_tenv fpf) ty fp
+Lemma get_owner_loc_footprint_map_wt ce: forall phl id fpm b ofs fp,
+    get_owner_loc_footprint_map (id, phl) fpm = OK (b, ofs, fp) ->
+    wt_fpm ce fpm ->
+    exists ty, wt_path ce (fpm_to_tenv fpm) (id, phl) = OK ty
+          /\ wt_footprint ce (fpm_to_tenv fpm) ty fp
           /\ (alignof ce ty | ofs).
 Admitted.
 
-Lemma get_owner_loc_footprint_frame_fp_ref_wf: forall sph fpf b ofs fp,
-    get_owner_loc_footprint_frame sph fpf = OK (b, ofs, fp) ->
-    fp_ref_loc_wf_fpf fpf ->
-    fp_ref_loc_wf fpf fp.
+Lemma get_owner_loc_footprint_map_fp_ref_wf: forall phl id fpm b ofs fp,
+    get_owner_loc_footprint_map (id, phl) fpm = OK (b, ofs, fp) ->
+    fp_ref_loc_wf_fpm fpm ->
+    fp_ref_loc_wf fpm fp.
 Admitted.
 
 
-Lemma get_owner_path_frame_inv: forall phl fid id (fpgf: fp_graph_frame) ph vs,
-    get_owner_path_frame (fid, (id, phl)) fpgf = OK (ph, vs) ->
-    exists fpm (fp: footprint),
-      nth_error fpgf fid = Some fpm
-      /\ fpm ! id = Some fp
-      /\ get_owner_path fpgf (fid, (id, nil)) phl fp nil = OK (ph, vs).
+Lemma get_owner_path_map_inv: forall id phl (fpg: fp_map) ph vs,
+    get_owner_path_map (id, phl) fpg = OK (ph, vs) ->
+    exists b ofs ty (fp: footprint),
+      fpg ! id = Some (b, ofs, ty, fp)
+      /\ get_owner_path fpg (id, nil) phl fp nil = OK (ph, vs).
 Admitted.
 
 (* If a path can be reached via (phl1 ++ phl2) then this reachable
 path can be divided into two parts: one is reached from phl1 and one
 is reach from phl2 *)
-Lemma get_owner_path_app_inv: forall phl1 phl2 ph1 ph3 sv1 vs1 vs3 (fpf: fp_frame),
-    get_owner_path fpf ph1 (phl1 ++ phl2) sv1 vs1 = OK (ph3, vs3) ->
+Lemma get_owner_path_app_inv: forall phl1 phl2 ph1 ph3 sv1 vs1 vs3 (fpm: fp_map),
+    get_owner_path fpm ph1 (phl1 ++ phl2) sv1 vs1 = OK (ph3, vs3) ->
     exists ph2 vs2 sv2,
-      get_owner_path fpf ph1 phl1 sv1 vs1 = OK (ph2, vs2) 
-      /\ get_owner_footprint_frame ph2 fpf = OK sv2 
-      /\ get_owner_path fpf ph2 phl2 sv2 vs2 = OK (ph3, vs3).
+      get_owner_path fpm ph1 phl1 sv1 vs1 = OK (ph2, vs2) 
+      /\ get_owner_footprint_map ph2 fpm = OK sv2 
+      /\ get_owner_path fpm ph2 phl2 sv2 vs2 = OK (ph3, vs3).
 Admitted.
 
-Lemma get_owner_path_for_owner: forall (fpf: fp_frame) ph fp,
-    get_owner_footprint_frame ph fpf = OK fp ->
+Lemma get_owner_path_for_owner: forall (fpm: fp_map) ph fp,
+    get_owner_footprint_map ph fpm = OK fp ->
     (* Since ph is an owner path, vs must only contain [ph] itself *)
-    get_owner_path_frame ph fpf = OK (ph, ph :: nil).
+    get_owner_path_map ph fpm = OK (ph, ph :: nil).
 Admitted.
 
-Lemma get_owner_loc_footprint_frame_eq: forall (fpf: fp_frame) ph b ofs fp,
-    get_owner_loc_footprint_frame ph fpf = OK (b, ofs, fp) ->
-    get_owner_footprint_frame ph fpf = OK fp.
+Lemma get_owner_loc_footprint_map_eq: forall (fpm: fp_map) ph b ofs fp,
+    get_owner_loc_footprint_map ph fpm = OK (b, ofs, fp) ->
+    get_owner_footprint_map ph fpm = OK fp.
 Admitted.
 
-Lemma get_owner_loc_footprint_frame_app: forall fid id phl1 phl2 b1 ofs1 fp1 b2 ofs2 fp2 (fpf: fp_frame),
-    get_owner_loc_footprint_frame (fid, (id, phl1)) fpf = OK (b1, ofs1, fp1) ->
+Lemma get_owner_loc_footprint_map_app: forall id phl1 phl2 b1 ofs1 fp1 b2 ofs2 fp2 (fpm: fp_map),
+    get_owner_loc_footprint_map (id, phl1) fpm = OK (b1, ofs1, fp1) ->
     get_owner_loc_footprint phl2 fp1 b1 ofs1 = OK (b2, ofs2, fp2) ->         
-    get_owner_loc_footprint_frame (fid, (id, phl1 ++ phl2)) fpf = OK (b2, ofs2, fp2).
+    get_owner_loc_footprint_map (id, phl1 ++ phl2) fpm = OK (b2, ofs2, fp2).
 Admitted.
 
 (** Misc for invalidate_conflict_ref and kill_paths *)
 
-Lemma get_owner_loc_footprint_frame_after_invalidate_ref: forall (fpf: fp_frame) ph1 ph2 ak am b ofs fp,
-    get_owner_loc_footprint_frame ph1 (invalidate_conflict_ref_fpf ph2 ak am fpf) = OK (b, ofs, fp) ->
-    exists fp', get_owner_loc_footprint_frame ph1 fpf = OK (b, ofs, fp')
+Lemma get_owner_loc_footprint_map_after_invalidate_ref: forall (fpm: fp_map) ph1 ph2 ak am b ofs fp,
+    get_owner_loc_footprint_map ph1 (invalidate_conflict_ref_fpm ph2 ak am fpm) = OK (b, ofs, fp) ->
+    exists fp', get_owner_loc_footprint_map ph1 fpm = OK (b, ofs, fp')
            /\ invalidate_conflict_ref ph2 ak am fp' = fp.
 Admitted.
 
-Lemma get_owner_path_frame_after_invalidate_ref: forall (fpf: fp_frame) ph1 ph2 ak am ph vs,
-    get_owner_path_frame ph1 (invalidate_conflict_ref_fpf ph2 ak am fpf) = OK (ph, vs) ->
-    get_owner_path_frame ph1 fpf = OK (ph, vs).
+Lemma get_owner_path_map_after_invalidate_ref: forall (fpm: fp_map) ph1 ph2 ak am ph vs,
+    get_owner_path_map ph1 (invalidate_conflict_ref_fpm ph2 ak am fpm) = OK (ph, vs) ->
+    get_owner_path_map ph1 fpm = OK (ph, vs).
 Admitted.
 
 
@@ -596,7 +584,7 @@ Let ge := globalenv se prog.
 (* composite environment *)
 Let ce := ge.(genv_cenv).
 
-Let wt_state := @wt_state ame prog se sg.
+(* Let wt_state := @wt_state ame prog se sg. *)
 
 (* Inductive borrowck_inv_cont: cont -> Prop := *)
 (* | borrowck_inv_cont_Kstop: borrowck_inv_cont Kstop *)
@@ -606,37 +594,38 @@ Let wt_state := @wt_state ame prog se sg.
 (* | borrowck_inv_cont_Kloop: forall s k *)
 (*     (CONT: borrowck_inv_cont k), *)
 (*     borrowck_inv_cont (Kloop s k) *)
-(* | borrowck_inv_cont_Kcall: forall k fpf p f *)
+(* | borrowck_inv_cont_Kcall: forall k fpm p f *)
 (*     (CONT: borrowck_inv_cont k) *)
 (*     (* We may require some invariant about that all views in *)
 (*     inout_paths must cover all reachable path of the inout_path in *)
 (*     fpm?  *) *)
-(*     (BOR_INV: borrow_check_inv fpf), *)
+(*     (** FIXME  *) *)
+(*     (BOR_INV: borrow_check_inv fpm), *)
 (*     borrowck_inv_cont (Kcall p f k). *)
 
 
 Inductive borrowck_inv : state -> Prop :=
-| borrowck_inv_regular_states: forall f s k fpm sup
+| borrowck_inv_regular_states: forall f s k fpm fidx sup
     (BOR_INV: borrow_check_inv fpm),
     (* (CONT: borrowck_inv_cont k), *)
-    borrowck_inv (State f s k fpm sup)
-| borrowck_inv_callstates: forall fid fpl inout_fpm sup k fd orgs org_rels tyargs tyres cconv
+    borrowck_inv (State f s k fpm fidx sup)
+| borrowck_inv_callstates: forall fid fpl fpm fidx sup k fd orgs org_rels tyargs tyres cconv
     (FINDF: ge.(genv_defmap) ! fid = Some (Gfun fd))
     (TYF: type_of_fundef fd = Tfunction orgs org_rels tyargs tyres cconv)
-    (BOR_INV: borrow_check_fpm_vals_inv inout_fpm fpl),
+    (BOR_INV: borrow_check_inv_snapshot fpm fpl),
     (* (CONT: borrowck_inv_cont k), *)
     (* (WTFP: list_forall2 (wt_footprint ce (fpm_to_tenv inout_fpm)) (type_list_of_typelist tyargs) fpl), *)
-    borrowck_inv (Callstate fid fpl inout_fpm sup k)
-| borrowck_inv_returnstates: forall rfp inout_fpm sup k rety
+    borrowck_inv (Callstate fid fpl fpm fidx sup k)
+| borrowck_inv_returnstates: forall rfp fpm fidx sup k rety
     (* The regions in the return type computed from cont are different
     from those in rety but it is not related to proving the invariant
     preservation. It is only related to proving the
     over-approximation? *)
     (RETY: typeof_cont_call (rs_sig_res sg) k = rety)
     (* (WTFP: wt_footprint ce (fpm_to_tenv inout_fpm) rety rfp) *)
-    (BOR_INV: borrow_check_fpm_vals_inv inout_fpm [rfp]),
+    (BOR_INV: borrow_check_inv_snapshot fpm [rfp]),
     (* (CONT: borrowck_inv_cont k), *)
-    borrowck_inv (Returnstate rfp inout_fpm sup k).
+    borrowck_inv (Returnstate rfp fpm fidx sup k).
 
 Ltac unfold_eval_assign :=
   match goal with
@@ -676,16 +665,12 @@ Definition access_kind_to_mut (ak: access_kind) : mutkind :=
 
 Coercion access_kind_to_mut : access_kind >-> mutkind.
 
-(** FIXME *)
-
-(*
-
 (* Thinking of its sufficiency to prove the borrow check invariant:
 the key point is to prove the stack discipline in the invariant. I
 think the two premises about the reachability in the borrow check
 invariant and the stack discipline field can be applied to this
 lemma? *)
-Lemma invalidate_conflict_ref_fpf_views_largest: forall phl1 id1 ak am (fpg1 fpg2: fp_graph)
+Lemma invalidate_conflict_ref_fpm_views_largest: forall phl1 id1 ak am (fpg1 fpg2: fp_map)
   (* Should we ensure that the mutability of (id1, phl1) (id2, phl2)
   match the access kind? How to dynamically check that all the deep
   path of (id1, phl1) is mutable? Maybe we do not need to check that
@@ -719,7 +704,7 @@ Lemma invalidate_conflict_ref_fpf_views_largest: forall phl1 id1 ak am (fpg1 fpg
   (VIEWS_INV: fp_graph_views_inv fpg1)
   (** TODO: define the spec of invalidae_conflict_ref_fpg for fpg2
   instead of mentioning fpg1 here *)
-  (INVALID: fpg2 = invalidate_conflict_ref_fpg (id1, phl1) ak am fpg1)
+  (INVALID: fpg2 = invalidate_conflict_ref_fpm (id1, phl1) ak am fpg1)
   phl2 id2 phl3 id3 vs2 vs3 tgt 
   (* We want to say that the views of (id2, phl2) are the largest
   view to its location *)
@@ -754,7 +739,7 @@ access_kind is irrelevant because we need to prove that the views of
 all reachable path from this accessed path cover all the mutable
 path. *)
 Lemma borrow_check_inv_deep_access: forall phl id (fpm1 fpm2: fp_map) fpl vs tgt b ofs fp ak
-    (BOR_INV: borrow_check_fpm_vals_inv fpm1 fpl)
+    (BOR_INV: borrow_check_inv_snapshot fpm1 fpl)
     (* wt_fpm ce fpm1 -> *)
     (* wt_footprint_list ce fpm1 tyl fpl -> *)
     (* wt_path ce (fpm_to_tenv fpm1) (id, phl) = OK ty -> *)
@@ -766,7 +751,7 @@ Lemma borrow_check_inv_deep_access: forall phl id (fpm1 fpm2: fp_map) fpl vs tgt
     (** We also need to invalidate fpl because some reference in fpl
     may be created by deeply accessing (id,phl)! This scenario is
     ruled out by the static borrow checking! *)
-    borrow_check_fpm_vals_inv fpm2 ((fp_ref ak b ofs (Some tgt) vs) :: (map (invalidate_conflict_ref (id, phl) ak BorrowCheckDomain.Adeep) fpl)).
+    borrow_check_inv_snapshot fpm2 ((fp_ref ak b ofs (Some tgt) vs) :: (map (invalidate_conflict_ref (id, phl) ak BorrowCheckDomain.Adeep) fpl)).
     (* /\ wt_footprint_list ce fpm2 ((Treference dummy_origin mut ty) :: tyl) ((fp_ref mut b ofs (Some tgt) vs) :: fpl) *)
     (* /\ wt_fpm ce fpm2. *)
 Proof.
@@ -784,45 +769,46 @@ Proof.
   with the above properties, we can extract this deep access path to a
   new temporary value. *)
   (* 1. The invariant is preserved by the invalidation process  *)
-  assert (BOR_INV1: borrow_check_fpm_vals_inv fpm2 (map (invalidate_conflict_ref (id, phl) ak Adeep) fpl)) by admit.
-  inv BOR_INV.
-  set (fpg1 := ((PTree_Properties.of_list
-                  (PTree.elements (fpm_to_fpg fpm1) ++
-                     combine (fresh_PTree_idents fpm1 (Datatypes.length fpl)) fpl)))) in *.  
-  inv BOR_INV1.
-  set (fpm2 := (invalidate_conflict_ref_fpm 
-                  (id, phl) ak Adeep fpm1)) in *.
-  set (fpl2 := (map
-                  (invalidate_conflict_ref 
-                     (id, phl) ak Adeep) fpl)) in *.
-  set (fpg2 := ((PTree_Properties.of_list
-                  (PTree.elements (fpm_to_fpg fpm2) ++
-                     combine (fresh_PTree_idents fpm2 (Datatypes.length fpl2)) fpl2)))) in *.
-  assert (FPG2: fpg2 = invalidate_conflict_ref_fpg (id, phl) ak Adeep fpg1) by admit.
-  (* 2. apply invalidate_conflict_ref_fpm_views_largest to show the
-  property of [vs] *)
-  generalize (invalidate_conflict_ref_fpm_views_largest phl id ak Adeep fpg1 fpg2 borrowck_views_inv_snapshot0 FPG2).
-  intros VS_TOP.
-  econstructor.
-  (* For now, ignore how to chose the new id *)
-  set (fresh_id := fresh_PTree_ident fpg2).
-  replace ((PTree_Properties.of_list
-       (PTree.elements (fpm_to_fpg fpm2) ++
-        combine
-          (fresh_PTree_idents fpm2
-             (Datatypes.length (fp_ref ak b ofs (Some tgt) vs :: fpl2)))
-          (fp_ref ak b ofs (Some tgt) vs :: fpl2)))) with (PTree.set fresh_id (fp_ref ak b ofs (Some tgt) vs) fpg2) by admit.
-  red.
-  (* Note: By case analysis, if both ph1 and ph2 do not include
-  fresh_id, then we use the invariant for fpg2; if ph1 or ph2 includes
-  fresh_id, then we use the property of
-  invalidate_conflict_ref_fpm_views_largest; if both ph1 and ph2
-  include fresh_id, then we may use the stack invariant in fpg2 to
-  show that the views created from traversing tgt to the tgt0 have
-  linear order.*)
-  admit.
-  admit.
-  admit.
+(*   assert (BOR_INV1: borrow_check_fpm_vals_inv fpm2 (map (invalidate_conflict_ref (id, phl) ak Adeep) fpl)) by admit. *)
+(*   inv BOR_INV. *)
+(*   set (fpg1 := ((PTree_Properties.of_list *)
+(*                   (PTree.elements (fpm_to_fpg fpm1) ++ *)
+(*                      combine (fresh_PTree_idents fpm1 (Datatypes.length fpl)) fpl)))) in *.   *)
+(*   inv BOR_INV1. *)
+(*   set (fpm2 := (invalidate_conflict_ref_fpm  *)
+(*                   (id, phl) ak Adeep fpm1)) in *. *)
+(*   set (fpl2 := (map *)
+(*                   (invalidate_conflict_ref  *)
+(*                      (id, phl) ak Adeep) fpl)) in *. *)
+(*   set (fpg2 := ((PTree_Properties.of_list *)
+(*                   (PTree.elements (fpm_to_fpg fpm2) ++ *)
+(*                      combine (fresh_PTree_idents fpm2 (Datatypes.length fpl2)) fpl2)))) in *. *)
+(*   assert (FPG2: fpg2 = invalidate_conflict_ref_fpg (id, phl) ak Adeep fpg1) by admit. *)
+(*   (* 2. apply invalidate_conflict_ref_fpm_views_largest to show the *)
+(*   property of [vs] *) *)
+(*   generalize (invalidate_conflict_ref_fpm_views_largest phl id ak Adeep fpg1 fpg2 borrowck_views_inv_snapshot0 FPG2). *)
+(*   intros VS_TOP. *)
+(*   econstructor. *)
+(*   (* For now, ignore how to chose the new id *) *)
+(*   set (fresh_id := fresh_PTree_ident fpg2). *)
+(*   replace ((PTree_Properties.of_list *)
+(*        (PTree.elements (fpm_to_fpg fpm2) ++ *)
+(*         combine *)
+(*           (fresh_PTree_idents fpm2 *)
+(*              (Datatypes.length (fp_ref ak b ofs (Some tgt) vs :: fpl2))) *)
+(*           (fp_ref ak b ofs (Some tgt) vs :: fpl2)))) with (PTree.set fresh_id (fp_ref ak b ofs (Some tgt) vs) fpg2) by admit. *)
+(*   red. *)
+(*   (* Note: By case analysis, if both ph1 and ph2 do not include *)
+(*   fresh_id, then we use the invariant for fpg2; if ph1 or ph2 includes *)
+(*   fresh_id, then we use the property of *)
+(*   invalidate_conflict_ref_fpm_views_largest; if both ph1 and ph2 *)
+(*   include fresh_id, then we may use the stack invariant in fpg2 to *)
+(*   show that the views created from traversing tgt to the tgt0 have *)
+(*   linear order.*) *)
+(*   admit. *)
+(*   admit. *)
+(*   admit. *)
+(* Admitted. *)
 Admitted.
 
 (* Move out the footprint pointed by the fp_ref in the temporary
@@ -837,12 +823,12 @@ use the invariant of fpm1; when both two path go through the moved out
 footprint, then we just construct their original path in fpm1 with the
 reference. *)
 Lemma borrow_check_inv_replace_move: forall (fpm1 fpm2: fp_map) fpl tgt b ofs fp,
-    borrow_check_fpm_vals_inv fpm1 ((fp_ref Mutable b ofs (Some tgt) [tgt]) :: fpl) ->
+    borrow_check_inv_snapshot fpm1 ((fp_ref Mutable b ofs (Some tgt) [tgt]) :: fpl) ->
     (* wt_fpm ce fpm1 -> *)
     (* wt_footprint_list ce fpm1 ((Treference r Mutable ty) :: tyl) ((fp_ref Mutable b ofs (Some tgt) vs) :: fpl) -> *)
     get_owner_loc_footprint_map tgt fpm1 = OK (b, ofs, fp) ->
     clear_footprint_map ce tgt fpm1 = OK fpm2 ->
-    borrow_check_fpm_vals_inv fpm2 (fp :: fpl).
+    borrow_check_inv_snapshot  fpm2 (fp :: fpl).
     (* /\ wt_footprint_list ce fpm2 (ty :: tyl) (fp :: fpl) *)
     (* /\ wt_fpm ce fpm2. *)
 Admitted.
@@ -850,10 +836,10 @@ Admitted.
 (* The borrow check invariant preserves when we drop any of the
 temporary footprint value. *)
 Lemma borrow_check_inv_drop: forall n (fpm: fp_map) fpl,
-    borrow_check_fpm_vals_inv fpm fpl ->
+    borrow_check_inv_snapshot fpm fpl ->
     (* wt_fpm ce fpm -> *)
     (* wt_footprint_list ce fpm tyl fpl -> *)
-    borrow_check_fpm_vals_inv fpm (list_delete n fpl).
+    borrow_check_inv_snapshot fpm (list_delete n fpl).
     (* /\ wt_footprint_list ce fpm (list_delete n tyl) (list_delete n fpl) *)
     (* /\ wt_fpm ce fpm. *)
 Admitted.
@@ -861,7 +847,7 @@ Admitted.
 (* Moving out a footprint: proved by borrow_check_inv_deep_access and
 borrow_check_inv_replace_move *)
 Lemma borrow_check_inv_move: forall (fpm1 fpm2 fpm3: fp_map) fpl tgt b ofs fp,
-    borrow_check_fpm_vals_inv fpm1 fpl ->
+    borrow_check_inv_snapshot fpm1 fpl ->
     (* wt_fpm ce fpm1 -> *)
     (* wt_footprint_list ce fpm1 tyl fpl -> *)
     (* wt_path ce (fpm_to_tenv fpm1) tgt = OK ty -> *)
@@ -874,7 +860,7 @@ Lemma borrow_check_inv_move: forall (fpm1 fpm2 fpm3: fp_map) fpl tgt b ofs fp,
     fpm2 = invalidate_conflict_ref_fpm tgt AWrite BorrowCheckDomain.Adeep fpm1 ->
     get_owner_loc_footprint_map tgt fpm2 = OK (b, ofs, fp) ->
     clear_footprint_map ce tgt fpm2 = OK fpm3 ->
-    borrow_check_fpm_vals_inv fpm3 (fp :: (map (invalidate_conflict_ref tgt AWrite BorrowCheckDomain.Adeep) fpl)).
+    borrow_check_inv_snapshot fpm3 (fp :: (map (invalidate_conflict_ref tgt AWrite BorrowCheckDomain.Adeep) fpl)).
     (* /\ wt_footprint_list ce fpm3 (ty :: tyl) (fp :: fpl) *)
     (* /\ wt_fpm ce fpm3. *)
 Proof.
@@ -900,7 +886,7 @@ be broken? Because when we set fp_uninit to some path, we should
 either invalidate the path point to the reachable path of this to-set
 path or kill the loans related to those reachable path? *)
 Lemma borrow_check_inv_shallow_write: forall (fpm1 fpm2 fpm3 fpm4: fp_map) id phl fpl vs tgt,
-    borrow_check_fpm_vals_inv fpm1 fpl ->
+    borrow_check_inv_snapshot fpm1 fpl ->
     (* wt_footprint_list ce fpm1 tyl fpl -> *)
     (* wt_fpm ce fpm1 -> *)
     (** Adhoc: we first do invalidation because we need to match the
@@ -914,12 +900,12 @@ Lemma borrow_check_inv_shallow_write: forall (fpm1 fpm2 fpm3 fpm4: fp_map) id ph
     (* This clearing operation is used to align with the kill loans operation. *)
     clear_footprint_map ce tgt fpm2 = OK fpm3 ->
     fpm4 = kill_paths_ref_fpm vs fpm3 ->
-    borrow_check_fpm_vals_inv fpm4 (map (kill_paths_ref vs) (map (invalidate_conflict_ref (id, phl) AWrite BorrowCheckDomain.Ashallow) fpl)).
+    borrow_check_inv_snapshot fpm4 (map (kill_paths_ref vs) (map (invalidate_conflict_ref (id, phl) AWrite BorrowCheckDomain.Ashallow) fpl)).
     (* /\ wt_footprint_list ce fpm4 tyl (map (kill_paths_ref vs) fpl) *)
     (* /\ wt_fpm ce fpm4. *)
 Proof.
   intros. subst.
-  unfold borrow_check_fpm_vals_inv in *.
+  (* unfold borrow_check_inv_snapshot in *. *)
   simpl in *.
   destruct H as [Hviews Hloc Hvals].
   econstructor.
@@ -932,13 +918,13 @@ Admitted.
 footprint is fp_emp or has been cleared by clear_footprint_map, and
 the invariant preserves. *)
 Lemma borrow_check_inv_set_fp: forall (fpm1 fpm2: fp_map) fpl tgt fp,
-    borrow_check_fpm_vals_inv fpm1 (fp :: fpl) ->
+    borrow_check_inv_snapshot fpm1 (fp :: fpl) ->
     (* wt_fpm ce fpm1 -> *)
     (* wt_footprint_list ce fpm1 (ty :: tyl) (fp :: fpl) -> *)
     check_path_is_dropped fpm1 tgt = OK true ->
     set_footprint_map tgt fp fpm1 = OK fpm2 ->
     (* wt_path ce (fpm_to_tenv fpm1) tgt = OK ty -> *)
-    borrow_check_fpm_vals_inv fpm2 fpl.
+    borrow_check_inv_snapshot fpm2 fpl.
     (* /\ wt_footprint_list ce fpm2 tyl fpl *)
     (* /\ wt_fpm ce fpm2. *)
 Admitted.
@@ -946,12 +932,12 @@ Admitted.
 (* moving from a place preserves the borrow checking invariant
 under the successful checking. But what is the effect of checking
 for pure expr? *)
-Lemma eval_expr_preserve_borchk_inv: forall (fpm1 fpm2: fp_map) e vfp
+Lemma eval_expr_preserve_borchk_inv: forall (fpm1 fpm2: fp_map) e vfp fidx
     (INV: borrow_check_inv fpm1)
     (* (WTFPM: wt_fpm ce fpm1) *)
     (* (WTEXPR: wt_expr (fpm_to_env fpm1) ce e) *)
-    (EVAL: eval_expr ce fpm1 e = OK (vfp, fpm2)),
-    borrow_check_fpm_vals_inv fpm2 [vfp].
+    (EVAL: eval_expr fidx ce fpm1 e = OK (vfp, fpm2)),
+    borrow_check_inv_snapshot fpm2 [vfp].
     (* /\ wt_fpm ce fpm2 *)
     (* /\ wt_footprint ce fpm2 (typeof e) vfp. *)
 Proof.
@@ -1017,15 +1003,14 @@ RustIRown *)
 (*     econstructor; eauto. *)
 (* Admitted. *)
    
-*) 
 
 End BORROWCK_INV.
 
 End ADT_ENV.
 
-Global Hint Resolve get_owner_loc_footprint_frame_wt
-  get_owner_loc_footprint_frame_fp_ref_wf
-  get_owner_path_frame_inv
+Global Hint Resolve get_owner_loc_footprint_map_wt
+  get_owner_loc_footprint_map_fp_ref_wf
+  get_owner_path_map_inv
   get_owner_path_for_owner
-  get_owner_loc_footprint_frame_eq
-  get_owner_loc_footprint_frame_app: fpmap.
+  get_owner_loc_footprint_map_eq
+  get_owner_loc_footprint_map_app: fpmap.
